Finished proofs in QhasmEvalCommon for formalizing mappings
Generalized and cleaned up state model

Generalized and cleaned up state model

src/Assembly/QhasmEvalCommon.v
@@ -3,251 +3,291 @@ Require Export ZArith Sumbool.
 Require Export Bedrock.Word.
 Require Import Logic.Eqdep_dec.
 
-Import State.
 Import Util.
 
-Definition evalTest {n} (o: TestOp) (a b: word n): bool :=
-  let c := (N.compare (wordToN a) (wordToN b)) in
+Module EvalUtil.
+  Definition evalTest {n} (o: TestOp) (a b: word n): bool :=
+    let c := (N.compare (wordToN a) (wordToN b)) in
 
-  let eqBit := match c with | Eq => true | _ => false end in
-  let ltBit := match c with | Lt => true | _ => false end in
-  let gtBit := match c with | Gt => true | _ => false end in
+    let eqBit := match c with | Eq => true | _ => false end in
+    let ltBit := match c with | Lt => true | _ => false end in
+    let gtBit := match c with | Gt => true | _ => false end in
 
-  match o with
-  | TEq => eqBit
-  | TLt => ltBit
-  | TLe => orb (eqBit) (ltBit)
-  | TGt => gtBit
-  | TGe => orb (eqBit) (gtBit)
-  end.
+    match o with
+    | TEq => eqBit
+    | TLt => ltBit
+    | TLe => orb (eqBit) (ltBit)
+    | TGt => gtBit
+    | TGe => orb (eqBit) (gtBit)
+    end.
 
-Definition evalCond (c: Conditional) (state: State): option bool :=
-  match c with
-  | CTrue => Some true
-  | CZero n r =>
-    omap (getReg r state) (fun v =>
-      if (Nat.eq_dec O (wordToNat v))
-      then Some true
-      else Some false) 
-  | CReg n o a b =>
-    omap (getReg a state) (fun va =>
-      omap (getReg b state) (fun vb =>
-        Some (evalTest o va vb)))
-  | CConst n o a c => 
-    omap (getReg a state) (fun va =>
-      Some (evalTest o va (constValueW c)))
-  end.
+  Definition evalIntOp {b} (io: IntOp) (x y: word b): (word b) * option bool :=
+    match io with
+    | Add =>
+      let v := (wordToN x + wordToN y)%N in
+      let c := (N.compare v (Npow2 b)) in
 
-Definition evalIntOp {b} (io: IntOp) (x y: word b): (word b) * option bool :=
-  match io with
-  | Add =>
-    let v := (wordToN x + wordToN y)%N in
-    let c := (N.compare v (Npow2 b)) in
+      match c as c' return c' = c -> _ with
+      | Lt => fun _ => (NToWord b v, Some false)
+      | _ => fun _ => (NToWord b v, Some true)
+      end eq_refl
 
-    match c as c' return c' = c -> _ with
-    | Lt => fun _ => (NToWord b v, Some false)
-    | _ => fun _ => (NToWord b v, Some true)
-    end eq_refl
+    | Sub => (wminus x y, None)
+    | Xor => (wxor x y, None)
+    | And => (wand x y, None)
+    | Or => (wor x y, None)
+    end.
 
-  | Sub => (wminus x y, None)
-  | Xor => (wxor x y, None)
-  | And => (wand x y, None)
-  | Or => (wor x y, None)
-  end.
+  Definition evalCarryOp {b} (io: CarryOp) (x y: word b) (c: bool): (word b) * bool :=
+    match io with
+    | AddWidthCarry =>
+      let v := (wordToN x + wordToN y + (if c then 1%N else 0%N))%N in
+      let c := (N.compare v (Npow2 b)) in
 
-Definition evalCarryOp {b} (io: CarryOp) (x y: word b) (c: bool): (word b) * bool :=
-  match io with
-  | AddWidthCarry =>
-    let v := (wordToN x + wordToN y + (if c then 1%N else 0%N))%N in
-    let c := (N.compare v (Npow2 b)) in
+      match c as c' return c' = c -> _ with
+      | Lt => fun _ => (NToWord b v, false)
+      | _ => fun _ => (NToWord b v, true)
+      end eq_refl
+    end.
 
-    match c as c' return c' = c -> _ with
-    | Lt => fun _ => (NToWord b v, false)
-    | _ => fun _ => (NToWord b v, true)
-    end eq_refl
-  end.
+  Definition evalDualOp {b} (duo: DualOp) (x y: word b) :=
+    match duo with
+    | Mult =>
+      let v := (wordToN x * wordToN y)%N in
+      let wres := NToWord (b + b) v in
+      (split1 b b wres, split2 b b wres)
+    end.
 
-Definition evalDualOp {b} (duo: DualOp) (x y: word b) :=
-  match duo with
-  | Mult =>
-    let v := (wordToN x * wordToN y)%N in
-    let wres := NToWord (b + b) v in
-    (split1 b b wres, split2 b b wres)
-  end.
+  Definition evalRotOp {b} (ro: RotOp) (x: word b) (n: nat) :=
+    match ro with
+    | Shl => NToWord b (N.shiftl_nat (wordToN x) n)
+    | Shr => NToWord b (N.shiftr_nat (wordToN x) n)
+    end.
 
-Definition evalRotOp {b} (ro: RotOp) (x: word b) (n: nat) :=
-  match ro with
-  | Shl => NToWord b (N.shiftl_nat (wordToN x) n)
-  | Shr => NToWord b (N.shiftr_nat (wordToN x) n)
-  end.
+  (* Width decideability *)
 
-Definition evalOperation (o: Operation) (state: State): option State :=
-  match o with
-  | IOpConst _ o r c =>
-    omap (getReg r state) (fun v =>
-      let (v', co) := (evalIntOp o v (constValueW c)) in
-      Some (setCarryOpt co (setReg r v' state)))
+  Definition getWidth (n: nat): option (Width n) :=
+    match n with
+    | 32 => Some W32
+    | 64 => Some W64
+    | _ => None
+    end.
 
-  | IOpReg _ o a b =>
-    omap (getReg a state) (fun va =>
-      omap (getReg b state) (fun vb =>
-        let (v', co) := (evalIntOp o va vb) in
-        Some (setCarryOpt co (setReg a v' state))))
+  Lemma getWidth_eq {n} (a: Width n): Some a = getWidth n.
+  Proof. induction a; unfold getWidth; simpl; intuition. Qed.
 
-  | IOpMem _ _ o r m i => 
-    omap (getReg r state) (fun va =>
-      omap (getMem m i state) (fun vb =>
-        let (v', co) := (evalIntOp o va vb) in
-        Some (setCarryOpt co (setReg r v' state))))
+  Lemma width_eq {n} (a b: Width n): a = b.
+  Proof. 
+    assert (Some a = Some b) as H by (
+      replace (Some a) with (getWidth n) by (rewrite getWidth_eq; intuition);
+      replace (Some b) with (getWidth n) by (rewrite getWidth_eq; intuition);
+      intuition).
+    inversion H; intuition.
+  Qed. 
 
-  | DOp _ o a b (Some x) => 
-    omap (getReg a state) (fun va =>
-      omap (getReg b state) (fun vb =>
-        let (low, high) := (evalDualOp o va vb) in
-        Some (setReg x high (setReg a low state))))
+  (* Mapping Conversions *)
 
-  | DOp _ o a b None => 
-    omap (getReg a state) (fun va =>
-      omap (getReg b state) (fun vb =>
-        let (low, high) := (evalDualOp o va vb) in
-        Some (setReg a low state)))
+  Definition wordToM {n: nat} {spec: Width n} (w: word n): Mapping n :=
+    constM _ (const spec w).
 
-  | ROp _ o r i => 
-    omap (getReg r state) (fun v =>
-      let v' := (evalRotOp o v i) in
-      Some (setReg r v' state))
+  Definition regToM {n: nat} {spec: Width n} (r: Reg n): Mapping n :=
+    regM _ r.
 
-  | COp _ o a b => 
-    omap (getReg a state) (fun va =>
-      omap (getReg b state) (fun vb =>
-        match (getCarry state) with
-        | None => None
-        | Some c0 => 
-          let (v', c') := (evalCarryOp o va vb c0) in
-          Some (setCarry c' (setReg a v' state))
-        end))
-  end.
+  Definition stackToM {n: nat} {spec: Width n} (s: Stack n): Mapping n :=
+    stackM _ s.
 
-Definition evalAssignment (a: Assignment) (state: State): option State :=
-  match a with
-  | ARegMem _ _ r m i => 
-    omap (getMem m i state) (fun v => Some (setReg r v state))
-  | AMemReg _ _ m i r =>
-    omap (getReg r state) (fun v => Some (setMem m i v state))
-  | AStackReg _ a b =>
-    omap (getReg b state) (fun v => Some (setStack a v state))
-  | ARegStack _ a b =>
-    omap (getStack b state) (fun v => Some (setReg a v state))
-  | ARegReg _ a b => 
-    omap (getReg b state) (fun v => Some (setReg a v state))
-  | AConstInt _ r c =>
-    Some (setReg r (constValueW c) state)
-  end.
+  Definition constToM {n: nat} {spec: Width n} (c: Const n): Mapping n :=
+    constM _ c.
 
-(* Width decideability *)
+  Definition mapping_dec {n} (a b: Mapping n): {a = b} + {a <> b}.
+    refine (match (a, b) as p' return (a, b) = p' -> _ with
+    | (regM v, regM v') => fun _ => 
+        if (Nat.eq_dec (regName v) (regName v'))
+        then left _
+        else right _
 
-Definition getWidth (n: nat): option (Width n) :=
-  match n with
-  | 32 => Some W32
-  | 64 => Some W64
-  | _ => None
-  end.
+    | (stackM v, stackM v') => fun _ => 
+        if (Nat.eq_dec (stackName v) (stackName v'))
+        then left _
+        else right _
 
-Lemma getWidth_eq {n} (a: Width n): Some a = getWidth n.
-Proof. induction a; unfold getWidth; simpl; intuition. Qed.
+    | (constM v, constM v') => fun _ => 
+        if (Nat.eq_dec (constValueN v) (constValueN v'))
+        then left _
+        else right _
 
-Lemma width_eq {n} (a b: Width n): a = b.
-Proof. 
-  assert (Some a = Some b) as H by (
-    replace (Some a) with (getWidth n) by (rewrite getWidth_eq; intuition);
-    replace (Some b) with (getWidth n) by (rewrite getWidth_eq; intuition);
-    intuition).
-  inversion H; intuition.
-Qed. 
+    | (memM _ v, memM _ v') => fun _ => 
+        if (Nat.eq_dec (memName v) (memName v')) 
+        then if (Nat.eq_dec (memLength v) (memLength v'))
+        then left _
+        else right _
+        else right _
 
-(* Mapping Conversions *)
+    | _ => fun _ => right _
+    end (eq_refl (a, b))); abstract (
+      inversion_clear _H;
+      unfold regName, stackName, constValueN, memName, memLength in *;
+      intuition; try inversion H;
+      destruct v, v'; subst;
+      try assert (w = w0) by (apply width_eq); do 3 first [
+          contradict _H0; inversion H1
+        | rewrite <- (natToWord_wordToNat w0);
+          rewrite <- (natToWord_wordToNat w2);
+          assert (w = w1) by (apply width_eq); subst;
+          rewrite _H0
+        | apply (inj_pair2_eq_dec _ Nat.eq_dec) in H3
+        | inversion H; subst; intuition
+        | intuition ]).
+  Defined.
 
-Definition wordToM {n: nat} {spec: Width n} (w: word n): Mapping n :=
-  constM _ (const spec w).
+  Definition dec_lt (a b: nat): {(a < b)%nat} + {(a >= b)%nat}.
+    assert ({(a <? b)%nat = true} + {(a <? b)%nat <> true})
+      by abstract (destruct (a <? b)%nat; intuition);
+      destruct H.
 
-Definition regToM {n: nat} {spec: Width n} (r: Reg n): Mapping n :=
-  regM _ r.
+    - left; abstract (apply Nat.ltb_lt in e; intuition).
 
-Definition stackToM {n: nat} {spec: Width n} (s: Stack n): Mapping n :=
-  stackM _ s.
+    - right; abstract (rewrite Nat.ltb_lt in n; intuition).
+  Defined.
 
-Definition constToM {n: nat} {spec: Width n} (c: Const n): Mapping n :=
-  constM _ c.
+  Fixpoint stackNames {n} (lst: list (Mapping n)): list nat :=
+    match lst with
+    | nil => nil
+    | cons c cs =>
+      match c with
+      | stackM v => cons (stackName v) (stackNames cs)
+      | _ => stackNames cs
+      end
+    end.
 
-Definition mapping_dec {n} (a b: Mapping n): {a = b} + {a <> b}.
-  refine (match (a, b) as p' return (a, b) = p' -> _ with
-  | (regM v, regM v') => fun _ => 
-    if (Nat.eq_dec (regName v) (regName v'))
-    then left _
-    else right _
+  Fixpoint regNames {n} (lst: list (Mapping n)): list nat :=
+    match lst with
+    | nil => nil
+    | cons c cs =>
+      match c with
+      | regM v => cons (regName v) (regNames cs)
+      | _ => regNames cs
+      end
+    end.
 
-  | (stackM v, stackM v') => fun _ => 
-    if (Nat.eq_dec (stackName v) (stackName v'))
-    then left _
-    else right _
+    (* Mapping Identifier-Triples *)
 
-  | (constM v, constM v') => fun _ => 
-    if (Nat.eq_dec (constValueN v) (constValueN v'))
-    then left _
-    else right _
+  Definition mappingId {n} (x: Mapping n): nat * nat * nat :=
+    match x with
+    | regM (reg n _ v) => (0, n, v)
+    | stackM (stack n _ v) => (1, n, v)
+    | constM (const n _ w) => (2, n, wordToNat w)
+    | memM _ (mem n m _ v) => (3, m, v)
+    end.
 
-  | (memM _ v, memM _ v') => fun _ => 
-    if (Nat.eq_dec (memName v) (memName v')) 
-    then if (Nat.eq_dec (memLength v) (memLength v'))
-      then left _
-      else right _
-    else right _
+  Lemma id_equal: forall {n: nat} (x y: Mapping n),
+    x = y <-> mappingId x = mappingId y.
+  Proof.
+    intros; split; intros; try abstract (rewrite H; intuition);
+      destruct x as [x | x | x | x], y as [y | y | y | y];
+      destruct x, y; unfold mappingId in H; simpl in H;
 
-  | _ => fun _ => right _
-  end (eq_refl (a, b))); abstract (
-    inversion_clear _H;
-    unfold regName, stackName, constValueN, memName, memLength in *;
-    intuition; try inversion H;
-    destruct v, v'; subst;
-    try assert (w = w0) by (apply width_eq); do 3 first [
-      contradict _H0; inversion H1
-    | rewrite <- (natToWord_wordToNat w0);
+      repeat match goal with
+      | [X: (_, _, _) = (_, _, _) |- _ ] =>
+        apply Triple_as_OT.conv in X
+      | [X: _ /\ _ /\ _ |- _ ] => destruct X
+      | [X: _ /\ _ |- _ ] => destruct X
+      | [A: Width _, B: Width _ |- _ ] =>
+        replace A with B by (apply width_eq)
+      | [X: context[match ?a with | _ => _ end] |- _ ] =>
+        destruct a
+      end; try subst; try omega; intuition.
+
+    rewrite <- (natToWord_wordToNat w0);
       rewrite <- (natToWord_wordToNat w2);
-      assert (w = w1) by (apply width_eq); subst;
-      rewrite _H0
-    | apply (inj_pair2_eq_dec _ Nat.eq_dec) in H3
-    | inversion H; subst; intuition
-    | intuition ]).
-Defined.
+      rewrite H1; intuition.
+  Qed.
 
-Definition dec_lt (a b: nat): {(a < b)%nat} + {(a >= b)%nat}.
-  assert ({(a <? b)%nat = true} + {(a <? b)%nat <> true})
-    by abstract (destruct (a <? b)%nat; intuition);
-    destruct H.
+  Definition id_dec := Triple_as_OT.eq_dec.
 
-  - left; abstract (apply Nat.ltb_lt in e; intuition).
+End EvalUtil.
 
-  - right; abstract (rewrite Nat.ltb_lt in n; intuition).
-Defined.
+Module QhasmEval.
+  Export EvalUtil FullState.
 
-Fixpoint stackNames {n} (lst: list (Mapping n)): list nat :=
-  match lst with
-  | nil => nil
-  | cons c cs =>
+  Definition evalCond (c: Conditional) (state: State): option bool :=
     match c with
-    | stackM v => cons (stackName v) (stackNames cs)
-    | _ => stackNames cs
-    end
-  end.
+    | CTrue => Some true
+    | CZero n r =>
+      omap (getReg r state) (fun v =>
+        if (Nat.eq_dec O (wordToNat v))
+        then Some true
+        else Some false) 
+    | CReg n o a b =>
+      omap (getReg a state) (fun va =>
+        omap (getReg b state) (fun vb =>
+          Some (evalTest o va vb)))
+    | CConst n o a c => 
+      omap (getReg a state) (fun va =>
+        Some (evalTest o va (constValueW c)))
+    end.
 
-Fixpoint regNames {n} (lst: list (Mapping n)): list nat :=
-  match lst with
-  | nil => nil
-  | cons c cs =>
-    match c with
-    | regM v => cons (regName v) (regNames cs)
-    | _ => regNames cs
-    end
-  end.
+  Definition evalOperation (o: Operation) (state: State): option State :=
+    match o with
+    | IOpConst _ o r c =>
+      omap (getReg r state) (fun v =>
+        let (v', co) := (evalIntOp o v (constValueW c)) in
+        Some (setCarryOpt co (setReg r v' state)))
 
+    | IOpReg _ o a b =>
+      omap (getReg a state) (fun va =>
+        omap (getReg b state) (fun vb =>
+            let (v', co) := (evalIntOp o va vb) in
+            Some (setCarryOpt co (setReg a v' state))))
 
+    | IOpMem _ _ o r m i => 
+      omap (getReg r state) (fun va =>
+        omap (getMem m i state) (fun vb =>
+            let (v', co) := (evalIntOp o va vb) in
+            Some (setCarryOpt co (setReg r v' state))))
+
+    | DOp _ o a b (Some x) => 
+      omap (getReg a state) (fun va =>
+        omap (getReg b state) (fun vb =>
+            let (low, high) := (evalDualOp o va vb) in
+            Some (setReg x high (setReg a low state))))
+
+    | DOp _ o a b None => 
+      omap (getReg a state) (fun va =>
+        omap (getReg b state) (fun vb =>
+            let (low, high) := (evalDualOp o va vb) in
+            Some (setReg a low state)))
+
+    | ROp _ o r i => 
+      omap (getReg r state) (fun v =>
+        let v' := (evalRotOp o v i) in
+        Some (setReg r v' state))
+
+    | COp _ o a b => 
+      omap (getReg a state) (fun va =>
+        omap (getReg b state) (fun vb =>
+            match (getCarry state) with
+            | None => None
+            | Some c0 => 
+            let (v', c') := (evalCarryOp o va vb c0) in
+            Some (setCarry c' (setReg a v' state))
+            end))
+    end.
+
+  Definition evalAssignment (a: Assignment) (state: State): option State :=
+    match a with
+    | ARegMem _ _ r m i => 
+      omap (getMem m i state) (fun v => Some (setReg r v state))
+    | AMemReg _ _ m i r =>
+      omap (getReg r state) (fun v => Some (setMem m i v state))
+    | AStackReg _ a b =>
+      omap (getReg b state) (fun v => Some (setStack a v state))
+    | ARegStack _ a b =>
+      omap (getStack b state) (fun v => Some (setReg a v state))
+    | ARegReg _ a b => 
+      omap (getReg b state) (fun v => Some (setReg a v state))
+    | AConstInt _ r c =>
+      Some (setReg r (constValueW c) state)
+    end.
+
+End QhasmEval.
